a first version of populate

theories/persistent/pstore_francois.v
@@ -71,28 +71,6 @@ Lemma lookup_insert_case `{Countable K} {V} (X:gmap K V) x y i :
   <[y:=i]> X !! x = if (decide (y=x)) then Some i else X !! x.
 Proof. case_decide; subst. rewrite lookup_insert //. rewrite lookup_insert_ne //. Qed.
 
-Lemma coherent_insert_bump M l ρ v σ :
-  dom_le ρ M ->
-  coherent ρ σ M ->
-  M !! (l, ρ) = Some v ->
-  coherent (S ρ) σ (<[(l, S ρ):=v]> M).
-Proof.
-  intros Hdom Hco ? l' ? E.
-  rewrite lookup_insert_case in E.
-  case_decide. naive_solver. exfalso.
-  apply elem_of_dom_2,Hdom in E. lia.
-Qed.
-
-Lemma dom_le_bump l ρ v M :
-  dom_le ρ M ->
-  dom_le (S ρ) (<[(l, S ρ):=v]> M).
-Proof.
-  intros Hd.
-  intros ??. rewrite dom_insert_L elem_of_union elem_of_singleton.
-  intros [X|X]; first naive_solver by lia.
-  apply Hd in X. lia.
-Qed.
-
 Lemma dom_le_update l ρ v M :
   dom_le ρ M ->
   dom_le ρ (<[(l, ρ):=v]> M).
@@ -103,27 +81,223 @@ Proof.
   apply Hd in X. lia.
 Qed.
 
-Lemma coherent_insert_unrel ρ' ρ σ M l v :
-  ρ ≠ ρ' ->
-  coherent ρ' σ M ->
-  coherent ρ' σ (<[(l, ρ):=v]> M).
+Definition interp_store (γ:gnames) ρ (σ:gmap location val) : iProp Σ :=
+  [∗ map] l ↦ v ∈ σ, mapsto γ ρ l v.
+
+Lemma interp_store_disj γ ρ σ1 σ2 :
+   interp_store γ ρ σ1 -∗ interp_store γ ρ σ2 -∗ ⌜σ1 ##ₘ σ2⌝.
 Proof.
-  intros Hcoh. intros ? l' v'.
-  rewrite lookup_insert_case. intros E.
-  case_decide; naive_solver.
+  rewrite /interp_store.
+  iIntros "E1 E2". iIntros (l).
+  destruct (σ1 !! l) eqn:X1, (σ2 !! l) eqn:X2; try done.
+  iDestruct (big_sepM_lookup with "[$]") as "?". done.
+  iDestruct (big_sepM_lookup with "[$]") as "?". done.
+  iDestruct (ghost_map_elem_frac_ne with "[$][$]") as "%".
+  { intros F. apply frac_valid in F. by compute in F. }
+  { exfalso. naive_solver. }
 Qed.
 
-Lemma pstore_capture_spec γ s ρ l v :
+(* For now, using the frac one of all points-tos, for the union to distribute.
+   We can do better. *)
+Lemma interp_store_union1 γ ρ σ1 σ2 :
+  interp_store γ ρ σ1 -∗ interp_store γ ρ σ2 -∗
+  interp_store γ ρ (σ1 ∪ σ2).
+Proof.
+  iIntros "? ?".
+  iDestruct (interp_store_disj with "[$][$]") as "%".
+  iApply big_sepM_union. done. by iFrame.
+Qed.
+
+Lemma interp_store_union2 γ ρ σ1 σ2 :
+  σ1 ##ₘ σ2 ->
+  interp_store γ ρ (σ1 ∪ σ2) -∗
+  interp_store γ ρ σ1 ∗ interp_store γ ρ σ2.
+Proof.
+  iIntros (?) "?". iApply big_sepM_union. done. by iFrame.
+Qed.
+
+Lemma interp_store_empty γ ρ :
+  interp_store γ ρ ∅ ≡ True%I.
+Proof.
+  rewrite /interp_store big_sepM_empty //.
+Qed.
+
+Lemma interp_store_singleton γ ρ l v :
+  interp_store γ ρ {[l:=v]} ≡ mapsto γ ρ l v.
+Proof.
+  rewrite /interp_store big_sepM_singleton //.
+Qed.
+
+Definition transportable γ (Φ:timestamp -> iProp Σ) : iProp Σ :=
+  ∀ (ρ:timestamp),
+    (Φ ρ -∗ ∃ (σ:gmap location val),
+        (interp_store γ ρ σ ∗
+         (interp_store γ ρ σ -∗ Φ ρ) ∗
+         (∀ ρ', interp_store γ ρ' σ -∗ Φ ρ'))).
+
+Lemma transportable_one γ l v :
+  ⊢ transportable γ (fun ρ => mapsto γ ρ l v).
+Proof.
+  iIntros (ρ). iIntros "?". iExists {[l:=v]}.
+  rewrite !interp_store_singleton. iIntros. iFrame.
+  iSplitR. iSteps. iIntros (?). rewrite interp_store_singleton. iSteps.
+Qed.
+
+Lemma transportable_persistent γ Φ :
+  ⊢ transportable γ (fun _ => □ Φ)%I.
+Proof.
+  iIntros (ρ). iIntros "#?". iExists ∅.
+  rewrite !interp_store_empty left_id.
+  iSplit. by iFrame "#". iIntros (?) "_". by iFrame "#".
+Qed.
+
+Lemma transportable_star γ Φ1 Φ2 :
+  transportable γ Φ1 -∗
+  transportable γ Φ2 -∗
+  transportable γ (fun ρ => Φ1 ρ ∗ Φ2 ρ)%I.
+Proof.
+  iIntros "F1 F2". iIntros (ρ) "(E1&E2)".
+  iDestruct ("F1" with "E1") as "[%σ1 (X11&X12&X13)]".
+  iDestruct ("F2" with "E2") as "[%σ2 (X21&X22&X23)]".
+  iDestruct (interp_store_disj with "X11 X21") as "%".
+  iDestruct (interp_store_union1 with "X11 X21") as "?".
+  iExists _. iFrame. iSplitL "X12 X22".
+  { iIntros "?".
+    iDestruct (interp_store_union2 with "[$]") as "(?&?)". done.
+    iSteps. }
+  { iIntros (?) "?".
+    iDestruct (interp_store_union2 with "[$]") as "(?&?)". done.
+    iSteps. }
+Qed.
+
+Lemma transportable_exists {A} γ Φ :
+  (∀ (x:A), transportable γ (Φ x) )-∗
+  transportable γ (fun ρ => ∃ x, Φ x ρ)%I.
+Proof.
+  iIntros "F". iIntros (?) "[%x H]".
+  iDestruct ("F" with "[$]") as "[% (?&X1&X2)]".
+  iExists _. iFrame. iSplitL "X1"; iSteps.
+Qed.
+
+(* XXX I don't know how to prove this. *)
+Lemma transportable_forall {A} γ Φ :
+  (∀ (x:A), transportable γ (Φ x) )-∗
+  transportable γ (fun ρ => ∀ x, Φ x ρ)%I.
+Abort.
+
+
+Definition submap (ρ:timestamp) (σ:gmap location val) (M:gmap (location*timestamp) val) :=
+  forall (l:location) (v:val), σ !! l = Some v -> M !! (l,ρ) = Some v.
+
+Lemma use_interp_store γ ρ σ M :
+  ghost_map_auth γ.(γ1) 1%Qp M -∗
+  interp_store γ ρ σ -∗
+  ⌜submap ρ σ M⌝.
+Proof.
+  iIntros "Ha Hf".
+  iIntros (l v Hlv).
+  iDestruct (big_sepM_lookup with "Hf") as "?". done.
+  iDestruct (ghost_map_lookup with "[$][$]") as "%". done.
+Qed.
+
+
+Definition news (ρ:timestamp) (σ:gmap location val)  : gmap (location*timestamp) val :=
+  kmap (fun l => (l,ρ)) σ.
+
+Lemma pureinv_disj_news ρ σ M xs μ :
+  pureinv ρ σ M xs ->
+  news (S ρ) μ ##ₘ M.
+Proof.
+  intros [X1 X2 X3 X4]. apply map_disjoint_spec.
+  intros (l,ρ') ? ? Hμ HM.
+  rewrite /news in Hμ.
+  apply lookup_kmap_Some in Hμ.
+  2:apply _. destruct Hμ as (l'&X&Hμ). inversion X. subst.
+  apply elem_of_dom_2,X4 in HM. lia.
+Qed.
+
+Lemma news_interp γ ρ μ :
+  ([∗ map] k↦v ∈ news ρ μ, k ↪[γ1 γ] v) -∗
+  interp_store γ ρ μ.
+Proof.
+  iIntros "Hm".
+  iInduction (μ) as [|] "IH" using map_ind.
+  { by iApply big_sepM_empty. }
+  { rewrite /interp_store.
+    rewrite /news kmap_insert !big_sepM_insert //.
+    { apply lookup_kmap_None. apply _. naive_solver. }
+    iDestruct "Hm" as "(?&?)". iFrame. iSteps. }
+Qed.
+
+Lemma dom_le_bump ρ μ M :
+  dom_le ρ M ->
+  dom_le (S ρ) (news (S ρ) μ ∪ M).
+Proof.
+  intros Hd.
+  intros ??. rewrite dom_union_L elem_of_union.
+  intros [X|X].
+  { rewrite /news dom_kmap in X. apply elem_of_map_1 in X.
+    naive_solver by lia. }
+  { apply Hd in X. lia. }
+Qed.
+
+Lemma lookup_news_Some ρ μ l ρ' v :
+  news ρ μ !! (l, ρ') = Some v ->
+  ρ' = ρ /\ μ !! l = Some v .
+Proof.
+  rewrite /news lookup_kmap_Some. naive_solver.
+Qed.
+
+Lemma coherent_insert_bump M ρ σ :
+  news (S ρ) σ ##ₘ M ->
+  dom_le ρ M ->
+  coherent ρ σ M ->
+  coherent (S ρ) σ (news (S ρ) σ ∪ M).
+Proof.
+  intros ? Hdom Hco l' ? E.
+  rewrite lookup_union_Some in E. done.
+  destruct E as [E|E].
+  { apply lookup_news_Some in E. naive_solver. }
+  { apply elem_of_dom_2,Hdom in E. lia. }
+Qed.
+
+Lemma coherent_insert_unrel ρ' ρ σ M μ :
+  news ρ μ ##ₘ M ->
+  ρ ≠ ρ' ->
+  coherent ρ' σ M ->
+  coherent ρ' σ (news ρ μ ∪ M).
+Proof.
+  intros ? Hcoh. intros ? l' v' E.
+  rewrite lookup_union_Some in E. done.
+  destruct E as [E|E].
+  { apply lookup_news_Some in E. naive_solver. }
+  { naive_solver. }
+Qed.
+
+
+Definition populate γ s ρ ρ' : iProp Σ :=
+  ∀ ρ0 Φ, isnow γ s ρ0 ∗ transportable γ Φ ∗ Φ ρ -∗ isnow γ s ρ0 ∗ Φ ρ ∗ Φ ρ'.
+
+Lemma interp_store_subseteq γ ρ σ σ' :
+  σ' ⊆ σ ->
+  interp_store γ ρ σ -∗
+  interp_store γ ρ σ'.
+Proof.
+  iIntros (?) "?".
+  by iApply (big_sepM_subseteq with "[$]").
+Qed.
+
+Lemma pstore_capture_spec γ s ρ :
     {{{
-      isnow γ s ρ ∗ mapsto γ ρ l v
+      isnow γ s ρ
     }}}
       pstore_capture s
     {{{ t ρ',
       RET t;
-      isnow γ s ρ' ∗ snapshot γ s t ρ ∗ mapsto γ ρ l v ∗ mapsto γ ρ' l v
+      isnow γ s ρ' ∗ snapshot γ s t ρ ∗ populate γ s ρ ρ'
     }}}.
 Proof.
-  iIntros (?) "(Hnow&Hmaps) Hpost".
+  iIntros (?) "Hnow Hpost".
   iDestruct "Hnow" as pat_now.
   iApply wp_fupd.
   wp_apply (pstore_capture_spec with "Hstore").
@@ -134,39 +308,51 @@ Proof.
   { rewrite lookup_app_r // Nat.sub_diag //. }
   iClear "HX".
 
-  iDestruct (ghost_map_lookup with "[$][$]") as "%".
-  iMod (ghost_map_insert (l,(S ρ)) v with "Hpointsto") as "(?&?)".
-  { destruct Hpure as [X1 X2 X3 X4]. apply not_elem_of_dom.
-    intros F. apply X4 in F. lia. }
+  assert (news (S ρ) σ ##ₘ M) by (eauto using pureinv_disj_news).
+  iMod (ghost_map_insert_big (news (S ρ) σ) with "[$]") as "(?&Hμ')".
+  { done. }
 
   iModIntro. iApply ("Hpost" $! t (S ρ)).
-  iFrame.
-  iSplitL.
-  2:{ destruct Hpure. subst. iExists _. iFrame "#". }
-  iExists _,_,_. iFrame. iPureIntro.
-  { destruct Hpure as [X1 X2 X3 X4].
+  iSplitR "Hμ'".
+  { iExists _,_,_. iFrame. iPureIntro.
+  { generalize Hpure. intros [X1 X2 X3 X4].
     constructor; eauto using coherent_insert_bump,dom_le_bump.
     { rewrite app_length //. simpl. lia. }
     { intros ??. rewrite lookup_app_Some. intros [?|(?&?)].
-      { eapply coherent_insert_unrel.
-        { apply lookup_lt_Some in H0. lia. }
-        { eauto. } }
+      { eapply coherent_insert_unrel; eauto.
+        { apply lookup_lt_Some in H0. lia. } }
       { apply list_lookup_singleton_Some in H1. destruct H1 as (?&<-).
         assert (ρ' = ρ) as -> by lia.
-        eauto using coherent_insert_unrel. } } }
+        eauto using coherent_insert_unrel. } } } }
+  iSplitR.
+  { destruct Hpure. subst. iExists _. iFrame "#". }
+  { erewrite <- pu1. 2:done. iIntros (ρ0 ϕ) "(Hnow&HT&?)".
+    iDestruct ("HT" with "[$]") as "[%σ' (X1&X2&X3)]".
+    clear dependent M. rename σ into σ_old. rename xs into xs_old.
+    iDestruct "Hnow" as pat_now.
+    iDestruct (use_interp_store with "Hpointsto [$]") as "%".
+    iSpecialize ("X2" with "[$]"). iFrame.
+    iAssert (⌜σ' ⊆ σ_old⌝)%I as "%Hsub".
+    { iDestruct (mono_list_lookup with "Hsnap [$]") as "%".
+      iPureIntro.
+      rewrite map_subseteq_spec. iIntros (l v Hl).
+      apply H in Hl. destruct Hpure as [X1 X2 X3 X4]. naive_solver. }
+    iDestruct (news_interp with "[$]") as "?".
+    iDestruct (interp_store_subseteq with "[$]") as "?". done.
+    iSpecialize ("X3" with "[$]"). iFrame. iExists _,_,_. by iFrame. }
 Qed.
 
-Lemma pstore_restore_spec γ s t ρ0 ρ l v :
+Lemma pstore_restore_spec γ s t ρ0 ρ :
     {{{
-      isnow γ s ρ0 ∗ snapshot γ s t ρ ∗ mapsto γ ρ l v
+      isnow γ s ρ0 ∗ snapshot γ s t ρ
     }}}
       pstore_restore s t
     {{{ ρ',
       RET ();
-      isnow γ s ρ' ∗ mapsto γ ρ l v ∗ mapsto γ ρ' l v
+      isnow γ s ρ' ∗ populate γ s ρ ρ'
     }}}.
 Proof.
-  iIntros (?) "(Hnow&Ht&E) Hpost".
+  iIntros (?) "(Hnow&Ht) Hpost".
   iDestruct "Hnow" as pat_now.
   iApply wp_fupd. rename σ into σ0.
 
@@ -177,31 +363,49 @@ Proof.
 
   iDestruct (mono_list_lookup with "Hsnap [$]") as "%".
   iMod (mono_list_update_app [σ0] with "Hsnap") as "Hsnap".
+  iDestruct (mono_list_lb_get with "Hsnap") as "#HX".
+  iDestruct (mono_list_elem_get (length xs) with "HX") as "#Hgo".
+  { rewrite lookup_app_r // Nat.sub_diag //. }
 
-  iDestruct (ghost_map_lookup with "[$][$]") as "%".
-  iMod (ghost_map_insert (l,(S ρ0)) v with "Hpointsto") as "(?&?)".
-  (* XXX lemma *)
-  { destruct Hpure as [X1 X2 X3 X4]. apply not_elem_of_dom.
-    intros F. apply X4 in F. lia. }
-  iFrame.
+  assert (news (S ρ0) σ ##ₘ M) by (eauto using pureinv_disj_news).
+  iMod (ghost_map_insert_big (news (S ρ0) σ) with "[$]") as "(?&Hμ')".
+  { done. }
 
-  iExists _,_,_. iFrame.
-  iPureIntro.
-  destruct Hpure as [X1 X2 X3 X4].
-  constructor; eauto using dom_le_bump.
-  { rewrite app_length. simpl. lia. }
-  { intros l' v' E.
-    rewrite lookup_insert_case in E. case_decide.
-    { inversion E. subst v. clear E.
-      assert (l'=l) by naive_solver. subst l'.
-      eapply X3; eauto. }
-    { exfalso. apply elem_of_dom_2,X4 in E. lia. } }
-  { intros ρ' σ'. rewrite lookup_app_Some. intros [X|(?&X)].
-    { eapply coherent_insert_unrel; eauto.
-      apply lookup_lt_Some in X. lia. }
-    { apply list_lookup_singleton_Some in X. destruct X as (?&<-).
-      assert (ρ' = ρ0) as -> by lia.
-      eauto using coherent_insert_unrel. } }
+  iModIntro. iSplitR "Hμ'".
+  { iExists _,_,_. iFrame.
+    iPureIntro.
+    destruct Hpure as [X1 X2 X3 X4].
+    constructor; eauto using dom_le_bump.
+    { rewrite app_length. simpl. lia. }
+    { intros l' v' E.
+      rewrite lookup_union_Some in E. done.
+      destruct E as [E|E].
+      { apply lookup_news_Some in E. naive_solver. }
+      { exfalso. apply elem_of_dom_2,X4 in E. lia. } }
+    { intros ρ' σ'. rewrite lookup_app_Some. intros [X|(?&X)].
+      { eapply coherent_insert_unrel; eauto.
+        apply lookup_lt_Some in X. lia. }
+      { apply list_lookup_singleton_Some in X. destruct X as (?&<-).
+        assert (ρ' = ρ0) as -> by lia.
+        eauto using coherent_insert_unrel. } } }
+  { erewrite <- pu1. 2:done. iIntros (? ϕ) "(Hnow&HT&?)".
+    iDestruct ("HT" with "[$]") as "[%σ' (X1&X2&X3)]".
+    clear dependent M. rename σ into σ_old. rename xs into xs_old.
+    iDestruct "Hnow" as pat_now.
+    iDestruct (use_interp_store with "Hpointsto [$]") as "%".
+    iSpecialize ("X2" with "[$]"). iFrame.
+    iAssert (⌜σ' ⊆ σ_old⌝)%I as "%Hsub".
+    { iDestruct (mono_list_lookup with "Hsnap [$]") as "%".
+      iDestruct (mono_list_lb_valid with "[$][$]") as "%Hprefix".
+      iPureIntro.
+      rewrite map_subseteq_spec. iIntros (l v Hl).
+      apply H0 in Hl. destruct Hpure as [X1 X2 X3 X4].
+      assert (xs_old !! ρ = xs !! ρ).
+      { apply prefix_lookup_lt. apply lookup_lt_Some in H. done. eauto using prefix_app_l. }
+      rewrite H2 in H. apply X3 in H. naive_solver. }
+    iDestruct (news_interp with "[$]") as "?".
+    iDestruct (interp_store_subseteq with "[$]") as "?". done.
+    iSpecialize ("X3" with "[$]"). iFrame. iExists _,_,_. by iFrame. }
 Qed.
 
 Lemma pstore_get_spec γ s ρ l v :
